LambdaS5/coq/LjsAuxiliary.v
@@ -1,0 +1,23 @@
+Generalizable All Variables.
+Set Implicit Arguments.
+Require Import LjsShared.
+Require Import Utils.
+Require Import LjsSyntax.
+
+Definition object_binds st ptr obj :=
+    Heap.binds (object_heap st) ptr obj.
+
+Definition object_indom st ptr :=
+    Heap.indom (object_heap st) ptr.
+
+Definition value_binds st loc v :=
+    Heap.binds (value_heap st) loc v.
+
+Definition value_indom st loc :=
+    Heap.indom (value_heap st) loc.
+
+Definition id_binds c i loc :=
+    Heap.binds (loc_heap c) i loc.
+
+Definition id_indom c i :=
+    Heap.indom (loc_heap c) i.
